Tweaks

Scratch.lean
@@ -78,3 +78,40 @@ noncomputable def toto {V : Type} : V ≃ quotient (⊥ : setoid V)
         left_inv := λ y, by { letI : setoid V := ⊥, exact quotient.eq.mp (quotient.out_eq ⟦y⟧) },
         right_inv := @quotient.out_eq V ⊥,
     }
+
+namespace tactic
+    meta def take_pi_args : nat → expr → list name
+    | (n+1) (expr.pi h _ _ e) := h :: take_pi_args n e
+    | _ _ := []
+
+    namespace interactive
+        setup_tactic_parser
+
+        meta def doneif (h : parse ident?) (t : parse (tk ":" *> texpr))
+                        (revert : parse ( (tk "generalizing" *> ((none <$ tk "*") <|> some <$> ident*)) <|> pure (some []))) :
+        tactic unit := do
+            let h := h.get_or_else `this,
+            t ← i_to_expr ``(%%t : Sort*),
+            (num_generalized, goal) ← retrieve (do
+                assert_core h t, swap,
+                num_generalized ← match revert with
+                | none := revert_all
+                | some revert := revert.mmap tactic.get_local >>= revert_lst
+                end,
+                goal ← target,
+                return (num_generalized, goal)),
+            tactic.assert h goal,
+            goal ← target,
+            (take_pi_args num_generalized goal).reverse.mmap' $ λ h,
+                try (tactic.get_local h >>= tactic.clear),
+            intron (num_generalized + 1)
+
+        meta def wlog' (h : parse ident?) (t : parse (tk ":" *> texpr)) : tactic unit :=
+        doneif h t none >> swap
+    end interactive
+end tactic
+
+example (n : ℤ) (h : ∃ p q : ℤ, n = p * q) : n*n ≥ 0 :=
+begin
+    rcases h with ⟨p,q,h⟩, wlog' : p ≥ 0,
+end
